Imp part 1.

Imp.v
@@ -182,5 +182,266 @@ Notation "'SKIP'" := CSkip.
 Notation "x '::=' c" := (CAss x c) (at level 60).
 Notation "c1 ;; c2" := (CSeq c1 c2) (at level 80, right associativity).
 Notation "'WHILE' b 'DO' c 'END'" := (CWhile b c) (at level 80, right associativity).
-Notation "'IFB' c1 'THEN' c2 'ELSE' c3" := (CIf c1 c2 c3)(at level 80, right associativity).
+Notation "'IFB' c1 'THEN' c2 'ELSE' c3 'FI'" := (CIf c1 c2 c3)(at level 80, right associativity).
 
+Fixpoint ceval_fun_no_while(st: state) (c:com) :state :=
+  match c with
+    | SKIP =>
+      st
+    | x ::= a1 =>
+      t_update st x (aeval st a1)
+    | c1 ;; c2 =>
+      let st' := ceval_fun_no_while st c1 in
+      ceval_fun_no_while st' c2
+    | IFB b THEN c1 ELSE c2 FI =>
+      if (beval st b)
+      then  ceval_fun_no_while st c1
+      else ceval_fun_no_while st c2
+    | WHILE b DO c END =>
+      st
+  end.
+
+
+Reserved Notation "c1 '/' st '\\' st'"
+         (at level 40, st at level 39).
+
+Inductive ceval : com -> state -> state -> Prop :=
+| E_Skip : forall st,
+             SKIP / st \\ st
+| E_Ass : forall st a1 n x,
+            aeval st a1 = n ->
+            (x ::= a1) / st \\ (t_update st x n)
+| E_Seq : forall c1 c2 st st' st'',
+            c1 / st \\ st' ->
+            c2 / st' \\ st'' ->
+            (c1 ;; c2) / st \\ st''
+| E_IfTrue : forall b c1 c2 st st',
+               (beval st b = true) ->
+               c1 / st \\ st' ->
+               (IFB b THEN c1 ELSE c2 FI) / st \\ st'
+| E_IfFalse :
+    forall b c1 c2 st st',
+      (beval st b = false) ->
+      c2 / st \\ st' ->
+      (IFB b THEN c1 ELSE c2 FI) / st \\ st'
+| E_WhileLoop :
+    forall b c st st' st'',
+      (beval st b = true) ->
+      c / st \\ st' ->
+      (WHILE b DO c END) / st' \\ st'' -> 
+      (WHILE b DO c END) / st \\ st''
+| E_WhileEnd :
+    forall b c st,
+      (beval st b = false) ->
+      (WHILE b DO c END) / st \\ st
+where "c1 '/' st '\\' st'" := (ceval c1 st st').
+
+Hint Resolve E_WhileLoop E_WhileEnd E_IfFalse E_IfTrue E_Seq E_Ass E_Skip : ceval_base.
+
+Example ceval_example1:
+  (X ::= ANum 2;;
+     IFB BLe (AId X) (ANum 1)
+     THEN Y ::= ANum 3
+     ELSE Z ::= ANum 4
+     FI) / empty_state \\ (t_update (t_update empty_state X 2) Z 4).
+Proof.
+  eapply E_Seq. eapply E_Ass. simpl; trivial.
+  simpl. eapply E_IfFalse; simpl. unfold t_update. rewrite eq_id_dec_id.
+  compute. trivial.
+  eapply E_Ass. simpl. trivial.
+Qed.
+
+Theorem ceval_determinstic:
+  forall c st st1 st2,
+    c / st \\ st1 ->
+    c / st \\ st2 ->
+    st1 = st2.
+  intros. generalize st2 H0. clear H0 st2.
+  elim H;  try (eauto with ceval_base).
+  intros. inversion H0; trivial.
+  intros. inversion H1. rewrite H0 in H6. rewrite H6; trivial.
+  intros. inversion H4. pose(H1 st'0 H7). apply H3. rewrite e. auto.
+  intros. inversion H3.  exact(H2 st2 H10). rewrite H9 in H0. inversion H0.
+  intros. inversion H3.  rewrite H9 in H0. inversion H0.
+  apply H2. auto.
+  intros. inversion H5. pose (H2 _ H9). rewrite <- e in H12. apply H4. auto.
+  rewrite H9 in H0. rewrite H10 in H0. inversion H0.
+  intros. inversion H1. rewrite H4 in H0; inversion H0. trivial.
+Qed.
+
+(*
+Theorem plus2_spec :
+  forall st n st',
+    st X = n ->
+    plus2 / st \\ st' ->
+    st' X = n + 2.*)
+
+Definition plus2 : com :=
+  X ::= (APlus (AId X) (ANum 2)).
+
+Definition XtimesYinZ : com :=
+  Z ::= (AMult (AId X) (AId Y)).
+
+Definition subtract_slowly_body : com :=
+  Z ::= AMinus (AId Z) (ANum 1) ;;
+    X ::= AMinus (AId X) (ANum 1).
+
+Definition subtract_slowly : com :=
+  WHILE BNot (BEq (AId X) (ANum 0)) DO
+        subtract_slowly_body
+        END.
+
+Definition subtract_3_from_5_slowly : com :=
+  X ::= ANum 3 ;;
+    Z ::= ANum 5 ;;
+    subtract_slowly.
+
+Definition loop : com :=
+  WHILE BTrue DO
+        SKIP
+        END.
+
+Theorem plus2_spec :
+  forall st n st',
+    st X = n ->
+    plus2 / st \\ st' ->
+    st' X = n + 2.
+  intros. unfold plus2 in H0. inversion H0. rewrite <- H5.
+  simpl. rewrite H. unfold t_update. apply eq_id_dec_id.
+Qed.
+
+
+Theorem XtimesYinZ_spec :
+  forall st n m st',
+    st X = n ->
+    st Y = m ->
+    XtimesYinZ / st \\ st' ->
+    st' Z = m * n.
+  unfold XtimesYinZ. intros.
+  inversion H1. rewrite <- H6 in H5. unfold t_update. rewrite eq_id_dec_id.
+  rewrite <- H6. simpl. rewrite H; rewrite H0. rewrite mult_comm. trivial.
+Qed.
+
+
+Theorem loop_never_stops:
+  forall c st st',
+    c=loop -> ~(loop / st \\ st').
+  unfold loop. unfold not. intros.
+  generalize H. elim H0; rewrite H; intros; try discriminate.
+  auto. inversion H2. rewrite <- H4 in H1. simpl in H1; discriminate.
+Qed.
+
+
+Fixpoint no_whiles (c:com) : bool :=
+  match c with
+    | SKIP =>
+      true
+    | _ ::= _ =>
+      true
+    | c1 ;; c2 =>
+      andb (no_whiles c1) (no_whiles c2)
+    | IFB _ THEN c1 ELSE c2 FI =>
+      andb (no_whiles c1) (no_whiles c2)
+    | WHILE _ DO _ END  =>
+      false
+  end.
+
+Inductive no_whilesR : com -> Prop :=
+| skip_nw : no_whilesR SKIP
+| ass_nw : forall a b, no_whilesR (a ::= b)
+| seq_nw : forall c1 c2, no_whilesR c1 -> no_whilesR c2 -> no_whilesR (c1 ;; c2)
+| if_nw : forall b c1 c2, no_whilesR c1 -> no_whilesR c2 -> no_whilesR (IFB b THEN c1 ELSE c2 FI).
+
+Theorem no_whiles_eqv :
+  forall c, no_whiles c = true <-> no_whilesR c.
+  split.
+  elim c; intros; try discriminate.
+  apply skip_nw. apply ass_nw. simpl in H1.
+  remember (no_whiles c0) as h1; remember (no_whiles c1) as h2.
+  generalize Heqh1 Heqh2; clear Heqh1 Heqh2.
+  case (no_whiles c0); case (no_whiles c1); intros hh hhh; try (rewrite hh in H1; rewrite hhh in H1; simpl in H1; inversion H1).
+  apply seq_nw; auto.
+  simpl in H1. remember (no_whiles c0) as h1; remember (no_whiles c1) as h2.
+  generalize Heqh1 Heqh2; clear Heqh1 Heqh2.
+  case (no_whiles c0); case (no_whiles c1); intros hh hhh; try (rewrite hh in H1; rewrite hhh in H1; simpl in H1; inversion H1).
+  apply if_nw; auto.
+  intros. elim H; intros; simpl; try auto.
+  rewrite H1; rewrite H3; try auto.
+  rewrite H1; rewrite H3; try auto.
+Qed.
+
+Print ex.
+
+Theorem no_whiles_terminating:
+  forall k, no_whilesR k -> forall st, exists st', k / st \\ st'.
+  intros k h.
+  elim h; intros.
+  exists st; apply E_Skip.
+  exists (t_update st a (aeval st b)). apply E_Ass. trivial.
+  pose (H0 st). inversion e. pose (H2 x). inversion e0.
+  exists x0. eapply E_Seq; eauto.
+  pose (H0 st). inversion e. pose (H2 st). inversion e0.
+  remember (beval st b) as c. generalize Heqc. clear Heqc.
+  case c; intros; [exists x; eapply E_IfTrue| exists x0; eapply E_IfFalse]; eauto.
+Qed.
+
+Inductive sinstr : Type :=
+| SPush : nat -> sinstr
+| SLoad : id -> sinstr
+| SPlus : sinstr
+| SMinus : sinstr
+| SMult : sinstr.
+
+
+Fixpoint s_execute (st : state)
+         (stack : list nat)
+         (prog : list sinstr) {struct prog} : list nat :=
+  match prog with
+    | nil => stack
+    | SPush x :: fol => s_execute st (x :: stack) fol
+    | SLoad a :: fol => s_execute st ((st a) :: stack) fol
+    | SPlus :: fol =>
+      match stack with
+        | x1::x2::newstack => s_execute st ((x1 + x2)::newstack) fol
+        | _ => s_execute st stack fol
+      end
+    | SMinus :: fol =>
+      match stack with
+        | x1::x2::newstack => s_execute st ((x2-x1)::newstack) fol
+        | _ => s_execute st stack fol
+      end
+    | SMult :: fol =>
+      match stack with
+        | x1 :: x2 :: newstack => s_execute st ((x1*x2)::newstack) fol
+        | _ => s_execute st stack fol
+      end
+  end.
+
+Example s_execute1:
+  s_execute empty_state []
+            [SPush 5; SPush 3; SPush 1; SMinus]
+  = [2;5]. auto.
+Qed.
+
+
+Example s_execute2:
+  s_execute (t_update empty_state X 3) [3;4]
+            [SPush 4; SLoad X; SMult; SPlus]
+  = [15;4].
+simpl. unfold t_update. rewrite eq_id_dec_id. auto.
+Qed.
+
+
+
+Fixpoint s_compile (e:aexp) : list sinstr :=
+  match e with
+    | ANum x => SPush x :: nil
+    | AId i => SLoad i :: nil
+    | APlus a b => (s_compile a) ++ (s_compile b) ++  SPlus :: nil
+    | AMinus a b => (s_compile a) ++ (s_compile b) ++ SMinus :: nil
+    | AMult a b => (s_compile a) ++ (s_compile b) ++ SMult :: nil
+  end.
+
+Theorem s_compile_correct :
+  forall st e,
+    s_execute st
